\item
A princípio, temos:
  \[{\chi ^2} = \sum\nolimits_{i,j} {\frac{{{{\left( {{N_{ij}} - {E_{ij}}} \right)}^2}}}{{{E_{ij}}}}} \]

e para facilitar a notação

\begin{center}
  \begin{tabular}{c c c}
    ${N_{++}} = \sum\nolimits_{i,j} {{N_{ij}}} $
    &
    ${{\hat p}_{ + j}} = \sum\nolimits_i {\frac{{{N_{ij}}}}{{{N_{ +  + }}}}} $
    &
    ${{\hat p}_{i + }} = \sum\nolimits_j {\frac{{{N_{ij}}}}{{{N_{ +  + }}}}} $
    \\
    ${{\hat p}_{ij}} = \frac{{{N_{ij}}}}{{{N_{ +  + }}}}$
    &
    ${E_{ij}} = {N_{ +  + }}{{\hat p}_{i + }}{{\hat p}_{ + j}}$
    &
    \\
  \end{tabular}
\end{center}

\begin{itemize}
  \item $\displaystyle{\chi ^2} = \sum\nolimits_{i,j} {\frac{{{{\left( {{N_{ij}} - {E_{ij}}} \right)}^2}}}{{{E_{ij}}}}}  = $
  \\
  $\displaystyle= \sum\nolimits_{i,j} {\frac{{{{\left( {{N_{ij}} - {N_{ +  + }}{{\hat p}_{i + }}{{\hat p}_{ + j}}} \right)}^2}}}{{{N_{ +  + }}{{\hat p}_{i + }}{{\hat p}_{ + j}}}}}  = \sum\nolimits_{i,j} {\frac{{{{\left( {{N_{ +  + }}\left( {{N_{ij}}/{N_{ +  + }} - {{\hat p}_{i + }}{{\hat p}_{ + j}}} \right)} \right)}^2}}}{{{N_{ +  + }}{{\hat p}_{i + }}{{\hat p}_{ + j}}}}}$
  \\
  $\displaystyle= \sum\nolimits_{i,j} {\frac{{{N_{ +  + }}^2}}{{{N_{ +  + }}}} \cdot \frac{{{{\left( {{N_{ij}}/{N_{ +  + }} - {{\hat p}_{i + }}{{\hat p}_{ + j}}} \right)}^2}}}{{{{\hat p}_{i + }}{{\hat p}_{ + j}}}}}  = {N_{ +  + }}\sum\nolimits_{i,j} {\frac{{{{\left( {{{\hat p}_{ij}} - {{\hat p}_{i + }}{{\hat p}_{ + j}}} \right)}^2}}}{{{{\hat p}_{i + }}{{\hat p}_{ + j}}}}}$

  \item $\displaystyle{\chi ^2} = \sum\nolimits_{i,j} {\frac{{{{\left( {{N_{ij}} - {E_{ij}}} \right)}^2}}}{{{E_{ij}}}}}  = $ \\
  \[\begin{array}{l}
  \displaystyle = \sum\nolimits_{i,j} {\frac{{{N_{ij}}^2 - 2{N_{ij}}{E_{ij}} + {E_{ij}}^2}}{{{E_{ij}}}}}  = \sum\nolimits_{i,j} {\frac{{{N_{ij}}^2}}{{{E_{ij}}}}}  + \sum\nolimits_{i,j} {\frac{{ - 2{N_{ij}}{E_{ij}}}}{{{E_{ij}}}}}  + \sum\nolimits_{i,j} {\frac{{{E_{ij}}^2}}{{{E_{ij}}}}} \\
  = \sum\nolimits_{i,j} {\frac{{{N_{ij}}^2}}{{{E_{ij}}}}}  - 2\underbrace {\sum\nolimits_{i,j} {{N_{ij}}} }_{{N_{ +  + }}} + \sum\nolimits_{i,j} {{E_{ij}}}  = \sum\nolimits_{i,j} {\frac{{{N_{ij}}^2}}{{{E_{ij}}}}}  - 2{N_{ +  + }} + \sum\nolimits_{i,j} {{N_{ +  + }}{{\hat p}_{i + }}{{\hat p}_{ + j}}} \\
  = \sum\nolimits_{i,j} {\frac{{{N_{ij}}^2}}{{{E_{ij}}}}}  - 2{N_{ +  + }} + {N_{ +  + }}\underbrace {\sum\nolimits_{i,j} {{{\hat p}_{i + }}{{\hat p}_{ + j}}} }_1 = \sum\nolimits_{i,j} {\frac{{{N_{ij}}^2}}{{{E_{ij}}}}}  - {N_{ +  + }}
  \end{array}\]
\end{itemize}
